@prefix ksa-ft: <https://w3id.org/ksa/feature-types/> .
@prefix ogc-ft: <http://www.opengis.net/def/metamodel/featuretypes/> .
@prefix owl: <http://www.w3.org/2002/07/owl#> .
@prefix rdfs: <http://www.w3.org/2000/01/rdf-schema#> .
@prefix skos: <http://www.w3.org/2004/02/skos/core#> .
@prefix xsd: <http://www.w3.org/2001/XMLSchema#> .

<https://w3id.org/ksa/feature-types/GeographicalNames/attribute/relatedSpatialObject> a owl:ObjectProperty,
        skos:Concept ;
    rdfs:label "relatedSpatialObject" ;
    rdfs:domain ksa-ft:PlaceName ;
    rdfs:range ksa-ft:AbstractFeatureType ;
    rdfs:subClassOf <https://w3id.org/ksa/feature-types/GeographicalNames/attribute> ;
    skos:broader <https://w3id.org/ksa/feature-types/GeographicalNames/attribute> .

ksa-ft:NameStatusValue a owl:Class,
        skos:Concept ;
    rdfs:label "Name Status Value"@en ;
    skos:broader <https://w3id.org/ksa/feature-types/GeographicalNames/codeLists> ;
    skos:definition "Code list for name status values of a geographical name"@en ;
    skos:inScheme ksa-ft:GeographicalNames .

ksa-ft:NativenessValue a owl:Class,
        skos:Concept ;
    rdfs:label "Nativeness Value"@en ;
    skos:broader <https://w3id.org/ksa/feature-types/GeographicalNames/codeLists> ;
    skos:definition "Code list for indication of nativeness of a geographical name"@en ;
    skos:inScheme ksa-ft:GeographicalNames .

ksa-ft:SpellingOfName a owl:Class,
        skos:Concept ;
    rdfs:label "Spelling Of Name"@en ;
    skos:broader <https://w3id.org/ksa/feature-types/GeographicalNames/codeLists> ;
    skos:definition "Proper way of spelling a name; the writing of a name with the correct capitalization and the correct letters and diacritics present in an accepted standard order."@en ;
    skos:inScheme ksa-ft:GeographicalNames .

ksa-ft:GeographicalName a owl:Class,
        skos:Concept ;
    rdfs:label "Geographical Name"@en ;
    skos:broader <https://w3id.org/ksa/feature-types/GeographicalNames/codeLists> ;
    skos:definition "Proper noun applied to a real world entity."@en ;
    skos:inScheme ksa-ft:GeographicalNames .

<https://w3id.org/ksa/feature-types/GeographicalNames/attribute/leastDetailedViewingResolution> a owl:DatatypeProperty,
        skos:Concept ;
    rdfs:label "leastDetailedViewingResolution"@en ;
    rdfs:domain ksa-ft:PlaceName ;
    rdfs:range xsd:integer ;
    rdfs:subClassOf <https://w3id.org/ksa/feature-types/GeographicalNames/attribute> ;
    skos:broader <https://w3id.org/ksa/feature-types/GeographicalNames/attribute> ;
    skos:definition """Resolution, expressed as the inverse of an indicative scale or a ground distance, above which the named place and its associated name(s) should no longer be displayed in a basic viewing service.

NOTE 1 This information may be used to determine if the names of the place name should be displayed at a given scale of display, only in the context of basic viewing services intending to show the content of the data set containing names. Even if this information is a valuable one for mapping in general, it is only approximate; cartographic services intending to produce high quality maps should certainly rely on other criteria and techniques for selecting names for the map.
NOTE 2 Even if this attribute is "voidable" for practical reasons linked to its availability in data sources, this information may be of first importance for viewing services. There are great chances that viewing services will inefficiently manage place names having this attribute void.

EXAMPLES The following examples use the equivalentScale attribute to express the attribute value.
- Names of important cities may be displayed at all viewing scales greater than 1/5,000,000. In this case, the value of the attribute is 5,000,000
- Names of small hamlets may only be displayed from all viewing scale greater than 1/25,000. In this case, the value of the attribute is 25,000
- Name of the country may be displayed at any small scale. In this case, this attribute is not filled.

NOTE 3 If the data set contain multiple representations of the same real world entity represented at different levels of detail, the scale ranges defined by the attributes leastDetailedViewingResolution and mostDetailedViewingResolution should not overlap, in order to avoid displaying the same names several times.

NOTE 4 The geometry of the named place should have a level of detail (i.e. resolution, granularity, precision, etc.) roughly compatible with its associated viewing scales."""@en ;
    skos:inScheme ksa-ft:GeographicalNames .

<https://w3id.org/ksa/feature-types/GeographicalNames/attribute/mostDetailedViewingResolution> a owl:DatatypeProperty,
        skos:Concept ;
    rdfs:label "mostDetailedViewingResolution"@en ;
    rdfs:domain ksa-ft:PlaceName ;
    rdfs:range xsd:integer ;
    rdfs:subClassOf <https://w3id.org/ksa/feature-types/GeographicalNames/attribute> ;
    skos:broader <https://w3id.org/ksa/feature-types/GeographicalNames/attribute> ;
    skos:definition """Resolution, expressed as the inverse of an indicative scale or a ground distance, below which the named place and its associated name(s) should no longer be displayed in a basic viewing service.

NOTE See description of leastDetailedViewingResolution

EXAMPLES The following examples use the equivalentScale attribute to express the attribute value.
- Names of wide areas like mountain ranges may not be displayed at all in viewing scales greater than 1/100,000. In this case, the value of the attribute is 100,000
- Names of small hamlets may be displayed at any large scale. In this case, this attribute is not filled."""@en ;
    skos:inScheme ksa-ft:GeographicalNames .

<https://w3id.org/ksa/feature-types/GeographicalNames/attribute/multiMediaImage> a owl:ObjectProperty,
        skos:Concept ;
    rdfs:label "multiMediaImage"@en ;
    rdfs:domain ksa-ft:PlaceName ;
    rdfs:subClassOf <https://w3id.org/ksa/feature-types/GeographicalNames/attribute> ;
    skos:broader <https://w3id.org/ksa/feature-types/GeographicalNames/attribute> ;
    skos:definition """An static visual that captures the characteristics of the specific geographical name

NOTE 1 One or more images can be attached to the specific geographical name to visually describe its characteristics.
NOTE 2 The image can be of form PNG

EXAMPLE In the case of a mountain name, the image of the mountain can be added"""@en ;
    skos:inScheme ksa-ft:GeographicalNames .

<https://w3id.org/ksa/feature-types/GeographicalNames/attribute/multiMediaVideo> a owl:ObjectProperty,
        skos:Concept ;
    rdfs:label "multiMediaVideo"@en ;
    rdfs:domain ksa-ft:PlaceName ;
    rdfs:subClassOf <https://w3id.org/ksa/feature-types/GeographicalNames/attribute> ;
    skos:broader <https://w3id.org/ksa/feature-types/GeographicalNames/attribute> ;
    skos:definition """An dynamic visual that captures the characteristics of the specific geographical name

NOTE One or more videos can be attached to the specific geographical name to visually describe its characteristics.
NOTE The image should be of format MP4

EXAMPLE In the case of a mountain name, the image of the mountain can be added"""@en ;
    skos:inScheme ksa-ft:GeographicalNames .

<https://w3id.org/ksa/feature-types/GeographicalNames/attribute/name> a owl:ObjectProperty,
        skos:Concept ;
    rdfs:label "name"@en ;
    rdfs:domain ksa-ft:PlaceName ;
    rdfs:range ksa-ft:GeographicalName ;
    rdfs:subClassOf <https://w3id.org/ksa/feature-types/GeographicalNames/attribute> ;
    skos:broader <https://w3id.org/ksa/feature-types/GeographicalNames/attribute> ;
    skos:definition "Name of the place name."@en ;
    skos:inScheme ksa-ft:GeographicalNames .

<https://w3id.org/ksa/feature-types/GeographicalNames/attribute/position> a owl:ObjectProperty,
        skos:Concept ;
    rdfs:label "position"@en ;
    rdfs:domain ksa-ft:PlaceName ;
    rdfs:subClassOf <https://w3id.org/ksa/feature-types/GeographicalNames/attribute> ;
    skos:broader <https://w3id.org/ksa/feature-types/GeographicalNames/attribute> ;
    skos:definition """Location associated to the named place. This data specification does not restrict the geometry types. 

NOTE 1 The most common geometry types for a named place are a reference point (modelled as GM_Point), a more precise geometry of the footprint (typically modelled as GM_Curve or GM_Surface), or a bounding box (to be modelled as a GM_Surface).
NOTE 2 If the geometry depicts the spatial footprint of the named place, a reference point and a bounding box could be derived from it. However, this specification does not require the explicit provision of any specific type of geometry such as bounding boxes or reference points.
NOTE 3 To avoid any misunderstanding, note that null geometry is not allowed by this specification.
NOTE 4 3D geometries are not really required for Geographical Names, but the model allows for it, so a data provider may publish it."""@en ;
    skos:inScheme ksa-ft:GeographicalNames .

<https://w3id.org/ksa/feature-types/GeographicalNames/attribute/type> a owl:ObjectProperty,
        skos:Concept ;
    rdfs:label "type"@en ;
    rdfs:domain ksa-ft:PlaceName ;
    rdfs:range ksa-ft:PlaceNameTypeValue ;
    rdfs:subClassOf <https://w3id.org/ksa/feature-types/GeographicalNames/attribute> ;
    skos:broader <https://w3id.org/ksa/feature-types/GeographicalNames/attribute> ;
    skos:definition """Characterization of the kind of entity designated by geographical name(s).

NOTE 1 This attribute should be consistent with the attribute 'relatedSpatialObject'. More precisely, if the attribute 'relatedSpatialObject' is filled in, the attribute 'type' should be filled in, and its value(s) should be consistent with the spatial data theme(s) of the related object(s).
NOTE 2 Even if this attribute may introduce some redundancy with the attribute 'relatedSpatialObject', it has to be filled in order to allow to use geographical names on their own without accessing to any other INSPIRE data set, which may be necessary in most cases."""@en ;
    skos:inScheme ksa-ft:GeographicalNames .

ksa-ft:PlaceNameTypeValue a owl:Class,
        skos:Concept ;
    rdfs:label "Place Name Type Value"@en ;
    skos:broader <https://w3id.org/ksa/feature-types/GeographicalNames/codeLists> ;
    skos:definition "Code list for the place name type value of a geographical name"@en ;
    skos:inScheme ksa-ft:GeographicalNames .

ksa-ft:AbstractFeatureType a owl:Class,
        skos:Concept ;
    rdfs:label "Abstract Feature Type"@en ;
    skos:definition "Abstract base Feature Type, which holds common attributes that are inherited by all Foundation Theme Feature Types."@en .

<https://w3id.org/ksa/feature-types/GeographicalNames/codeLists> a owl:Class,
        skos:Concept ;
    rdfs:label "Geographical Names Foundation Theme code list or type"@en ;
    skos:inScheme ksa-ft:GeographicalNames .

ksa-ft:PlaceName a owl:Class,
        skos:Concept ;
    rdfs:label "Place Name"@en ;
    ogc-ft:hasProperty <https://w3id.org/ksa/feature-types/GeographicalNames/attribute/leastDetailedViewingResolution>,
        <https://w3id.org/ksa/feature-types/GeographicalNames/attribute/mostDetailedViewingResolution>,
        <https://w3id.org/ksa/feature-types/GeographicalNames/attribute/multiMediaImage>,
        <https://w3id.org/ksa/feature-types/GeographicalNames/attribute/multiMediaVideo>,
        <https://w3id.org/ksa/feature-types/GeographicalNames/attribute/name>,
        <https://w3id.org/ksa/feature-types/GeographicalNames/attribute/position>,
        <https://w3id.org/ksa/feature-types/GeographicalNames/attribute/type> ;
    rdfs:subClassOf ksa-ft:AbstractFeatureType ;
    skos:broader ksa-ft:AbstractFeatureType ;
    skos:definition "Any real world entity referred to by one or several proper nouns."@en ;
    skos:inScheme ksa-ft:GeographicalNames .

ksa-ft:GeographicalNames a skos:ConceptScheme ;
    rdfs:label "Geographical Names Foundation Theme"@en ;
    skos:definition "Geographical Names provide cultural, historical and political orientation and identity to geographical places with one or more official or unofficial names. They are location identifiers for man-made and natural features of the real world, such as districts, regions or any feature of public or historical interest."@en .

<https://w3id.org/ksa/feature-types/GeographicalNames/attribute> a owl:Class,
        skos:Concept ;
    rdfs:label "Geographical Names Foundation Theme attribute"@en ;
    skos:inScheme ksa-ft:GeographicalNames .

