@prefix geoNames: <https://w3id.org/ksa/feature-types/GeographicalNames/> .
@prefix ksa-ft: <https://w3id.org/ksa/feature-types/> .
@prefix owl: <http://www.w3.org/2002/07/owl#> .
@prefix rdfs: <http://www.w3.org/2000/01/rdf-schema#> .
@prefix skos: <http://www.w3.org/2004/02/skos/core#> .

geoNames:GeographicalName a owl:Class,
        skos:Concept ;
    rdfs:label "Geographical Name"@en ;
    skos:broader geoNames:codeLists ;
    skos:definition "Proper noun applied to a real world entity."@en ;
    skos:inScheme ksa-ft:GeographicalNames ;
    skos:prefLabel "Geographical Name"@en .

geoNames:NameStatusValue a owl:Class,
        skos:Concept ;
    rdfs:label "Name Status Value"@en ;
    skos:broader geoNames:codeLists ;
    skos:definition "Code list for name status values of a geographical name"@en ;
    skos:inScheme ksa-ft:GeographicalNames ;
    skos:prefLabel "Name Status Value"@en .

geoNames:NativenessValue a owl:Class,
        skos:Concept ;
    rdfs:label "Nativeness Value"@en ;
    skos:broader geoNames:codeLists ;
    skos:definition "Code list for indication of nativeness of a geographical name"@en ;
    skos:inScheme ksa-ft:GeographicalNames ;
    skos:prefLabel "Nativeness Value"@en .

geoNames:PlaceNameTypeValue a owl:Class,
        skos:Concept ;
    rdfs:label "Place Name Type Value"@en ;
    skos:broader geoNames:codeLists ;
    skos:definition "Code list for the place name type value of a geographical name"@en ;
    skos:inScheme ksa-ft:GeographicalNames ;
    skos:prefLabel "Place Name Type Value"@en .

geoNames:SpellingOfName a owl:Class,
        skos:Concept ;
    rdfs:label "Spelling Of Name"@en ;
    skos:broader geoNames:codeLists ;
    skos:definition "Proper way of spelling a name; the writing of a name with the correct capitalization and the correct letters and diacritics present in an accepted standard order."@en ;
    skos:inScheme ksa-ft:GeographicalNames ;
    skos:prefLabel "Spelling Of Name"@en .

geoNames:codeLists a owl:Class,
        skos:Concept ;
    rdfs:label "Geographical Names Foundation Theme code list or type"@en ;
    skos:inScheme ksa-ft:GeographicalNames ;
    skos:prefLabel "Geographical Names Foundation Theme code list or type"@en .

ksa-ft:GeographicalNames a skos:ConceptScheme ;
    rdfs:label "Geographical Names Foundation Theme"@en ;
    skos:definition "Geographical Names provide cultural, historical and political orientation and identity to geographical places with one or more official or unofficial names. They are location identifiers for man-made and natural features of the real world, such as districts, regions or any feature of public or historical interest."@en ;
    skos:prefLabel "Geographical Names Foundation Theme"@en .

