@prefix ksa-ft: <https://w3id.org/ksa/feature-types/> .
@prefix ogc-ft: <http://www.opengis.net/def/metamodel/featuretypes/> .
@prefix owl: <http://www.w3.org/2002/07/owl#> .
@prefix rdfs: <http://www.w3.org/2000/01/rdf-schema#> .
@prefix skos: <http://www.w3.org/2004/02/skos/core#> .
@prefix xsd: <http://www.w3.org/2001/XMLSchema#> .

ksa-ft:ImageAggregation a owl:Class,
        skos:Concept ;
    rdfs:label "Image Aggregation"@en ;
    skos:broader <https://w3id.org/ksa/feature-types/Imagery/codeLists> ;
    skos:definition "Geometrical characteristics of the image aggregation."@en ;
    skos:inScheme ksa-ft:Imagery .

ksa-ft:InterpolationMethodValue a owl:Class,
        skos:Concept ;
    rdfs:label "Interpolation Method"@en ;
    skos:broader <https://w3id.org/ksa/feature-types/Imagery/codeLists> ;
    skos:definition """List of codes that identify the interpolation methods which may be used for evaluating orthoimage coverages.

NOTE 1 This Saudi NSDI-governed code list is derived from the code list CV_InterpolationMethod specified in ISO 19123. CV_InterpolationMethod is not used  as such because not actually implemented.

NOTE 2 Example values: nearestneighbor, bilinear, biquadratic, bicubic, etc..."""@en ;
    skos:inScheme ksa-ft:Imagery .

ksa-ft:TerrestrialImageShapeTypeValue a owl:Class,
        skos:Concept ;
    rdfs:label "Terrestrial Image Shape Type"@en ;
    skos:broader <https://w3id.org/ksa/feature-types/Imagery/codeLists> ;
    skos:definition "The shape type of the terrestrial image."@en ;
    skos:inScheme ksa-ft:Imagery .

ksa-ft:ViewVolume a owl:Class,
        skos:Concept ;
    rdfs:label "View Volume"@en ;
    skos:broader <https://w3id.org/ksa/feature-types/Imagery/codeLists> ;
    skos:definition "Specify what is the horizontal and vertical field of view of the image."@en ;
    skos:inScheme ksa-ft:Imagery .

ksa-ft:Attitude a owl:Class,
        skos:Concept ;
    rdfs:label "Attitude"@en ;
    skos:broader <https://w3id.org/ksa/feature-types/Imagery/codeLists> ;
    skos:definition "Values describing orientation of the satellite at the given moment in time."@en ;
    skos:inScheme ksa-ft:Imagery .

ksa-ft:Ephemeris a owl:Class,
        skos:Concept ;
    rdfs:label "Ephemeris"@en ;
    skos:broader <https://w3id.org/ksa/feature-types/Imagery/codeLists> ;
    skos:definition "Position and velocity of the satellite at specific point in time. Position and velocity should be specified in the same Coordinate Reference System and in 3D."@en ;
    skos:inScheme ksa-ft:Imagery .

ksa-ft:ExteriorOrientation a owl:Class,
        skos:Concept ;
    rdfs:label "Exterior Orientation"@en ;
    skos:broader <https://w3id.org/ksa/feature-types/Imagery/codeLists> ;
    skos:definition "Elements of the exterior orientation of the camera. The Coordinate Reference System is specified by the Coordinate Reference System of the nodal point."@en ;
    skos:inScheme ksa-ft:Imagery .

<https://w3id.org/ksa/feature-types/Imagery/attribute/GSD> a owl:ObjectProperty,
        skos:Concept ;
    rdfs:label "GSD"@en ;
    rdfs:domain ksa-ft:SpaceborneImage ;
    rdfs:subClassOf <https://w3id.org/ksa/feature-types/Imagery/attribute> ;
    skos:broader <https://w3id.org/ksa/feature-types/Imagery/attribute> ;
    skos:definition "Coarse specification of the distance between pixels' centres."@en ;
    skos:inScheme ksa-ft:Imagery .

<https://w3id.org/ksa/feature-types/Imagery/attribute/RPCs> a owl:DatatypeProperty,
        skos:Concept ;
    rdfs:label "RPCs"@en ;
    rdfs:domain ksa-ft:SpaceborneImage ;
    rdfs:range xsd:decimal ;
    rdfs:subClassOf <https://w3id.org/ksa/feature-types/Imagery/attribute> ;
    skos:broader <https://w3id.org/ksa/feature-types/Imagery/attribute> ;
    skos:definition "Rational polynomial coefficients."@en ;
    skos:inScheme ksa-ft:Imagery .

<https://w3id.org/ksa/feature-types/Imagery/attribute/attitude> a owl:ObjectProperty,
        skos:Concept ;
    rdfs:label "attitude"@en ;
    rdfs:domain ksa-ft:SpaceborneImage ;
    rdfs:range ksa-ft:Attitude ;
    rdfs:subClassOf <https://w3id.org/ksa/feature-types/Imagery/attribute> ;
    skos:broader <https://w3id.org/ksa/feature-types/Imagery/attribute> ;
    skos:definition "Values describing orientation of the satellite at the given moment in time."@en ;
    skos:inScheme ksa-ft:Imagery .

<https://w3id.org/ksa/feature-types/Imagery/attribute/auxFile> a owl:ObjectProperty,
        skos:Concept ;
    rdfs:label "auxFile"@en ;
    rdfs:domain ksa-ft:DepthMap ;
    rdfs:subClassOf <https://w3id.org/ksa/feature-types/Imagery/attribute> ;
    skos:broader <https://w3id.org/ksa/feature-types/Imagery/attribute> ;
    skos:definition "Aux file associated with this depth map."@en ;
    skos:inScheme ksa-ft:Imagery .

<https://w3id.org/ksa/feature-types/Imagery/attribute/environmentalConditions> a owl:ObjectProperty,
        skos:Concept ;
    rdfs:label "environmentalConditions"@en ;
    rdfs:domain ksa-ft:ObliqueAirborneImage ;
    rdfs:subClassOf <https://w3id.org/ksa/feature-types/Imagery/attribute> ;
    skos:broader <https://w3id.org/ksa/feature-types/Imagery/attribute> ;
    skos:definition "Description of environmental conditions like: wind, temperature, humidity etc."@en ;
    skos:inScheme ksa-ft:Imagery .

<https://w3id.org/ksa/feature-types/Imagery/attribute/ephemeris> a owl:ObjectProperty,
        skos:Concept ;
    rdfs:label "ephemeris"@en ;
    rdfs:domain ksa-ft:SpaceborneImage ;
    rdfs:range ksa-ft:Ephemeris ;
    rdfs:subClassOf <https://w3id.org/ksa/feature-types/Imagery/attribute> ;
    skos:broader <https://w3id.org/ksa/feature-types/Imagery/attribute> ;
    skos:definition "Ephemeris of the satellite during creating the image."@en ;
    skos:inScheme ksa-ft:Imagery .

<https://w3id.org/ksa/feature-types/Imagery/attribute/exteriorOrientation> a owl:ObjectProperty,
        skos:Concept ;
    rdfs:label "exteriorOrientation"@en ;
    rdfs:domain ksa-ft:ObliqueAirborneImage ;
    rdfs:range ksa-ft:ExteriorOrientation ;
    rdfs:subClassOf <https://w3id.org/ksa/feature-types/Imagery/attribute> ;
    skos:broader <https://w3id.org/ksa/feature-types/Imagery/attribute> ;
    skos:definition "Elements of the exterior orientation of the camera."@en ;
    skos:inScheme ksa-ft:Imagery .

<https://w3id.org/ksa/feature-types/Imagery/attribute/flightHeight> a owl:ObjectProperty,
        skos:Concept ;
    rdfs:label "flightHeight"@en ;
    rdfs:domain ksa-ft:ObliqueAirborneImage ;
    rdfs:subClassOf <https://w3id.org/ksa/feature-types/Imagery/attribute> ;
    skos:broader <https://w3id.org/ksa/feature-types/Imagery/attribute> ;
    skos:definition "Height of the flight."@en ;
    skos:inScheme ksa-ft:Imagery .

<https://w3id.org/ksa/feature-types/Imagery/attribute/mosaicExtent> a owl:ObjectProperty,
        skos:Concept ;
    rdfs:label "mosaicExtent"@en ;
    rdfs:domain ksa-ft:MosaicElement ;
    rdfs:subClassOf <https://w3id.org/ksa/feature-types/Imagery/attribute> ;
    skos:broader <https://w3id.org/ksa/feature-types/Imagery/attribute> ;
    skos:definition """Geometric representation spatially delineating the date and time of acquisition of the several input images that contribute to the final mosaic.

NOTE The boundaries of the geometries are commonly based on the seamlines used for the mosaicking process."""@en ;
    skos:inScheme ksa-ft:Imagery .

<https://w3id.org/ksa/feature-types/Imagery/attribute/phenomenonTime> a owl:ObjectProperty,
        skos:Concept ;
    rdfs:label "phenomenonTime"@en ;
    rdfs:domain ksa-ft:MosaicElement ;
    rdfs:subClassOf <https://w3id.org/ksa/feature-types/Imagery/attribute> ;
    skos:broader <https://w3id.org/ksa/feature-types/Imagery/attribute> ;
    skos:definition """Description of the observation/acquisition extent in time of the input image(s).

NOTE 1 This temporal extent refers to the interval of time in which the input image(s) was/were acquired by the sensor.

NOTE 2 When the acquisition is considered as instantaneous, despite the exposure time, the end date and time can be identical to the begin date and time.

EXAMPLE 1 begin: 2011-10-30 end: 2011-10-30

EXAMPLE 2 begin: 2011-06-07T14:31:02Z end: 2011-06-07T16:10:54Z."""@en ;
    skos:inScheme ksa-ft:Imagery .

<https://w3id.org/ksa/feature-types/Imagery/attribute/scale> a owl:DatatypeProperty,
        skos:Concept ;
    rdfs:label "scale"@en ;
    rdfs:domain ksa-ft:SpaceborneImage ;
    rdfs:range xsd:decimal ;
    rdfs:subClassOf <https://w3id.org/ksa/feature-types/Imagery/attribute> ;
    skos:broader <https://w3id.org/ksa/feature-types/Imagery/attribute> ;
    skos:definition "Scale of the image."@en ;
    skos:inScheme ksa-ft:Imagery .

<https://w3id.org/ksa/feature-types/Imagery/attribute/segFile> a owl:ObjectProperty,
        skos:Concept ;
    rdfs:label "segFile"@en ;
    rdfs:domain ksa-ft:DepthMap ;
    rdfs:subClassOf <https://w3id.org/ksa/feature-types/Imagery/attribute> ;
    skos:broader <https://w3id.org/ksa/feature-types/Imagery/attribute> ;
    skos:definition "Seg file associated with this depth map."@en ;
    skos:inScheme ksa-ft:Imagery .

ksa-ft:DepthMap a owl:Class,
        skos:Concept ;
    rdfs:label "Depth Map"@en ;
    ogc-ft:hasProperty <https://w3id.org/ksa/feature-types/Imagery/attribute/auxFile>,
        <https://w3id.org/ksa/feature-types/Imagery/attribute/segFile> ;
    rdfs:subClassOf ksa-ft:AbstractTerrestrialImage ;
    skos:broader ksa-ft:AbstractTerrestrialImage ;
    skos:definition "Raster dataset representing distance between camera and specific spatial elements in the image. This type of dataset can be derived from LIDAR."@en ;
    skos:inScheme ksa-ft:Imagery .

ksa-ft:MosaicElement a owl:Class,
        skos:Concept ;
    rdfs:label "Mosaic Element"@en ;
    ogc-ft:hasProperty <https://w3id.org/ksa/feature-types/Imagery/attribute/mosaicExtent>,
        <https://w3id.org/ksa/feature-types/Imagery/attribute/phenomenonTime> ;
    rdfs:subClassOf ksa-ft:AbstractFeatureType ;
    skos:broader ksa-ft:AbstractFeatureType ;
    skos:definition "Abstract type identifying both the contributing area and the acquisition time of one or several input images used to generate a mosaiced orthoimage coverage. The main purpose of this feature type is the provision of a mechanism for describing the spatial distribution of the acquisition dates and times over a mosaiced orthoimage. The acquisition time can be supplied either for each individual input image, or for sets of input images grouped together according to temporal criteria."@en ;
    skos:inScheme ksa-ft:Imagery .

ksa-ft:ObliqueAirborneImage a owl:Class,
        skos:Concept ;
    rdfs:label "Oblique Airborne Image"@en ;
    ogc-ft:hasProperty <https://w3id.org/ksa/feature-types/Imagery/attribute/environmentalConditions>,
        <https://w3id.org/ksa/feature-types/Imagery/attribute/exteriorOrientation>,
        <https://w3id.org/ksa/feature-types/Imagery/attribute/flightHeight> ;
    rdfs:subClassOf ksa-ft:Image ;
    skos:broader ksa-ft:Image ;
    skos:definition "Image of the Earth surface intentionally captured at a very high offpointing angle for specific applications from aircraft (plane, UAV, helicopter etc.)."@en ;
    skos:inScheme ksa-ft:Imagery .

ksa-ft:SpaceborneImage a owl:Class,
        skos:Concept ;
    rdfs:label "Spaceborne Image"@en ;
    ogc-ft:hasProperty <https://w3id.org/ksa/feature-types/Imagery/attribute/GSD>,
        <https://w3id.org/ksa/feature-types/Imagery/attribute/RPCs>,
        <https://w3id.org/ksa/feature-types/Imagery/attribute/attitude>,
        <https://w3id.org/ksa/feature-types/Imagery/attribute/ephemeris>,
        <https://w3id.org/ksa/feature-types/Imagery/attribute/scale> ;
    rdfs:subClassOf ksa-ft:Image ;
    skos:broader ksa-ft:Image ;
    skos:definition "Raster image of the Earth surface that was acquired using spaceborne platform (e.g. satellite)."@en ;
    skos:inScheme ksa-ft:Imagery .

<https://w3id.org/ksa/feature-types/Imagery/codeLists> a owl:Class,
        skos:Concept ;
    rdfs:label "Imagery Foundation Theme code list or type"@en ;
    skos:inScheme ksa-ft:Imagery .

<https://w3id.org/ksa/feature-types/Imagery/attribute> a owl:Class,
        skos:Concept ;
    rdfs:label "Imagery Foundation Theme attribute"@en ;
    skos:inScheme ksa-ft:Imagery .

ksa-ft:Imagery a skos:ConceptScheme ;
    rdfs:label "Imagery Foundation Theme"@en ;
    skos:definition "The Imagery Foundation Theme is a suite of continuously updated georeferenced spaceborne, airborne and terrestrial imagery, as well as any novel sources, for the Kingdom of Saudi Arabia. The Foundation Theme makes imagery with different resolutions available nationally to multiple users for a wide range of missions such as national security, natural resource management and urban development."@en .

