@prefix ksa-ft: <https://w3id.org/ksa/feature-types/> .
@prefix landUse: <https://w3id.org/ksa/feature-types/LandUse/> .
@prefix landUse-att: <https://w3id.org/ksa/feature-types/LandUse/attribute/> .
@prefix ogc-ft: <http://www.opengis.net/def/metamodel/featuretypes/> .
@prefix owl: <http://www.w3.org/2002/07/owl#> .
@prefix rdfs: <http://www.w3.org/2000/01/rdf-schema#> .
@prefix skos: <http://www.w3.org/2004/02/skos/core#> .
@prefix xsd: <http://www.w3.org/2001/XMLSchema#> .

landUse:DateType a owl:Class,
        skos:Concept ;
    rdfs:label "Date Type"@en ;
    skos:broader landUse:codeLists ;
    skos:definition "Reference date and event of lifecycle/process stage of spatial plan document used to describe it."@en ;
    skos:inScheme ksa-ft:LandUse ;
    skos:prefLabel "Date Type"@en .

landUse:LandUseClassificationValue a owl:Class,
        skos:Concept ;
    rdfs:label "Land Use Classification"@en ;
    skos:broader landUse:codeLists ;
    skos:definition "List of land use classes to be used in The Kingdom."@en ;
    skos:inScheme ksa-ft:LandUse ;
    skos:prefLabel "Land Use Classification"@en .

landUse:LandUsePercentage a owl:Class,
        skos:Concept ;
    rdfs:label "Land Use Percentage"@en ;
    skos:broader landUse:codeLists ;
    skos:definition "Percentage of a land use object that is covered by a presence."@en ;
    skos:inScheme ksa-ft:LandUse ;
    skos:prefLabel "Land Use Percentage"@en .

landUse:OwnershipTypeValue a owl:Class,
        skos:Concept ;
    rdfs:label "Ownership Type"@en ;
    skos:broader landUse:codeLists ;
    skos:definition "Type of ownership."@en ;
    skos:inScheme ksa-ft:LandUse ;
    skos:prefLabel "Ownership Type"@en .

landUse:ParcelLandUseValue a owl:Class,
        skos:Concept ;
    rdfs:label "Parcel Land Use Value"@en ;
    skos:broader landUse:codeLists ;
    skos:definition "Land Use information within the parcel object."@en ;
    skos:inScheme ksa-ft:LandUse ;
    skos:prefLabel "Parcel Land Use Value"@en .

landUse:ProcessStepGeneralValue a owl:Class,
        skos:Concept ;
    rdfs:label "Process Step General"@en ;
    skos:broader landUse:codeLists ;
    skos:definition "General indication of the step of the planning process that the plan is undergoing."@en ;
    skos:inScheme ksa-ft:LandUse ;
    skos:prefLabel "Process Step General"@en .

landUse:RegulationNatureValue a owl:Class,
        skos:Concept ;
    rdfs:label "Regulation Nature"@en ;
    skos:broader landUse:codeLists ;
    skos:inScheme ksa-ft:LandUse ;
    skos:prefLabel "Regulation Nature"@en .

landUse:RoadSurfaceCategoryValue a owl:Class,
        skos:Concept ;
    rdfs:label "Road Surface Catagory"@en ;
    skos:broader landUse:codeLists ;
    skos:definition "Values to indicate whether a road is paved or not paved."@en ;
    skos:inScheme ksa-ft:LandUse ;
    skos:prefLabel "Road Surface Catagory"@en .

landUse:SpatialPlanTypeValue a owl:Class,
        skos:Concept ;
    rdfs:label "Spatial Plan Type"@en ;
    skos:broader landUse:codeLists ;
    skos:definition "Type of spatial plan document."@en ;
    skos:inScheme ksa-ft:LandUse ;
    skos:prefLabel "Spatial Plan Type"@en .

landUse:UrbanBoundaryTypeValue a owl:Class,
        skos:Concept ;
    rdfs:label "Urban Boundary Type"@en ;
    skos:broader landUse:codeLists ;
    skos:definition "Type of urban boundary."@en ;
    skos:inScheme ksa-ft:LandUse ;
    skos:prefLabel "Urban Boundary Type"@en .

landUse:VerticalLandUse a owl:Class,
        skos:Concept ;
    rdfs:label "Vertical Land Use"@en ;
    skos:broader landUse:codeLists ;
    skos:definition "Land Use classes that are present in a specific vertical level of using of a parcel object."@en ;
    skos:inScheme ksa-ft:LandUse ;
    skos:prefLabel "Vertical Land Use"@en .

landUse:VerticalLevelValue a owl:Class,
        skos:Concept ;
    rdfs:label "Vertical Level"@en ;
    skos:broader landUse:codeLists ;
    skos:definition "The relative vertical level of a land use of a parcel object."@en ;
    skos:inScheme ksa-ft:LandUse ;
    skos:prefLabel "Vertical Level"@en .

landUse-att:additionalDescription a owl:ObjectProperty,
        skos:Concept ;
    rdfs:label "additionalDescription"@en ;
    rdfs:domain landUse:MapDocument ;
    rdfs:subClassOf landUse:attribute ;
    skos:broader landUse:attribute ;
    skos:definition "Plain text description of additional information not fitting in other attributes."@en ;
    skos:inScheme ksa-ft:LandUse ;
    skos:prefLabel "additionalDescription"@en .

landUse-att:coordinateReferenceSystem a owl:ObjectProperty,
        skos:Concept ;
    rdfs:label "coordinateReferenceSystem"@en ;
    rdfs:domain landUse:MapDocument ;
    rdfs:subClassOf landUse:attribute ;
    skos:broader landUse:attribute ;
    skos:definition """Identifier and codespace for coordinate reference system of map document.

NOTE. Refer to EPSG Geodetic Parameter Dataset  (EPSG) as URI identifier of reference system e.g.  http://www.opengis.net/def/crs/EPSG/0/4326"""@en ;
    skos:inScheme ksa-ft:LandUse ;
    skos:prefLabel "coordinateReferenceSystem"@en .

landUse-att:extent a owl:ObjectProperty,
        skos:Concept ;
    rdfs:label "extent"@en ;
    rdfs:domain landUse:ExistingLandUseCollection ;
    rdfs:subClassOf landUse:attribute ;
    skos:broader landUse:attribute ;
    skos:definition """Contains the extent of the data set.

NOTE 01. For an area objects boundary of the geometrical union of all the instances of the spatial object type ExistingLandUseUnit.
For an sampled objects the convex hull of all the instances of the spatial object type ExistingLandUseUnit."""@en ;
    skos:inScheme ksa-ft:LandUse ;
    skos:prefLabel "extent"@en .

landUse-att:legend a owl:ObjectProperty,
        skos:Concept ;
    rdfs:label "legend"@en ;
    rdfs:domain landUse:MapDocument ;
    rdfs:subClassOf landUse:attribute ;
    skos:broader landUse:attribute ;
    skos:definition "Link to online version of legend of map document."@en ;
    skos:inScheme ksa-ft:LandUse ;
    skos:prefLabel "legend"@en .

landUse-att:link a owl:ObjectProperty,
        skos:Concept ;
    rdfs:label "link"@en ;
    rdfs:domain landUse:MapDocument ;
    rdfs:subClassOf landUse:attribute ;
    skos:broader landUse:attribute ;
    skos:definition "Link to online version of map document."@en ;
    skos:inScheme ksa-ft:LandUse ;
    skos:prefLabel "link"@en .

landUse-att:name a owl:DatatypeProperty,
        skos:Concept ;
    rdfs:label "name"@en ;
    rdfs:domain landUse:ExistingLandUseCollection ;
    rdfs:range xsd:string ;
    rdfs:subClassOf landUse:attribute ;
    skos:broader landUse:attribute ;
    skos:definition "Name of the Land Use collection"@en ;
    skos:inScheme ksa-ft:LandUse ;
    skos:prefLabel "name"@en .

landUse-att:spatialResolution a owl:DatatypeProperty,
        skos:Concept ;
    rdfs:label "spatialResolution"@en ;
    rdfs:domain landUse:MapDocument ;
    rdfs:range xsd:integer ;
    rdfs:subClassOf landUse:attribute ;
    skos:broader landUse:attribute ;
    skos:definition "Level of detail expressed as an integer value expressing the scale denominator of a comparable hardcopy map."@en ;
    skos:inScheme ksa-ft:LandUse ;
    skos:prefLabel "spatialResolution"@en .

landUse-att:title a owl:DatatypeProperty,
        skos:Concept ;
    rdfs:label "title"@en ;
    rdfs:domain landUse:MapDocument ;
    rdfs:range xsd:string ;
    rdfs:subClassOf landUse:attribute ;
    skos:broader landUse:attribute ;
    skos:definition "Official title of the map document."@en ;
    skos:inScheme ksa-ft:LandUse ;
    skos:prefLabel "title"@en .

landUse-att:validFrom a owl:DatatypeProperty,
        skos:Concept ;
    rdfs:label "validFrom"@en ;
    rdfs:domain landUse:ExistingLandUseCollection,
        landUse:MapDocument ;
    rdfs:range xsd:date ;
    rdfs:subClassOf landUse:attribute ;
    skos:broader landUse:attribute ;
    skos:definition "First date at which the map document is valid in reality."@en,
        "The date when the Land Use data set started to exist in the real world."@en ;
    skos:inScheme ksa-ft:LandUse ;
    skos:prefLabel "validFrom"@en .

landUse-att:validTo a owl:DatatypeProperty,
        skos:Concept ;
    rdfs:label "validTo"@en ;
    rdfs:domain landUse:ExistingLandUseCollection,
        landUse:MapDocument ;
    rdfs:range xsd:date ;
    rdfs:subClassOf landUse:attribute ;
    skos:broader landUse:attribute ;
    skos:definition "The dwte from which the Land Use data set no longer exists in the real world."@en,
        "The time from which the map document no longer exists in the real world."@en ;
    skos:inScheme ksa-ft:LandUse ;
    skos:prefLabel "validTo"@en .

landUse:ExistingLandUseCollection a owl:Class,
        skos:Concept ;
    rdfs:label "Existing Land Use Collection"@en ;
    ogc-ft:hasProperty landUse-att:extent,
        landUse-att:name,
        landUse-att:validFrom,
        landUse-att:validTo ;
    rdfs:subClassOf <https://w3id.org/ksa/feature-types/BaseTypes/AbstractFeatureType> ;
    skos:broader <https://w3id.org/ksa/feature-types/BaseTypes/AbstractFeatureType> ;
    skos:definition "A collection of units (areas or locations) for which information on existing land use is provided as a polygon."@en ;
    skos:inScheme ksa-ft:LandUse ;
    skos:prefLabel "Existing Land Use Collection"@en .

landUse:MapDocument a owl:Class,
        skos:Concept ;
    rdfs:label "Map Document"@en ;
    ogc-ft:hasProperty landUse-att:additionalDescription,
        landUse-att:coordinateReferenceSystem,
        landUse-att:legend,
        landUse-att:link,
        landUse-att:spatialResolution,
        landUse-att:title,
        landUse-att:validFrom,
        landUse-att:validTo ;
    rdfs:subClassOf <https://w3id.org/ksa/feature-types/BaseTypes/AbstractFeatureType> ;
    skos:broader <https://w3id.org/ksa/feature-types/BaseTypes/AbstractFeatureType> ;
    skos:definition "The scanned plan and structural drawing which may geo-referenced e.g. raster images, vector drawings."@en ;
    skos:inScheme ksa-ft:LandUse ;
    skos:prefLabel "Map Document"@en .

landUse:codeLists a owl:Class,
        skos:Concept ;
    rdfs:label "Land Use Foundation Theme code list or type"@en ;
    skos:inScheme ksa-ft:LandUse ;
    skos:prefLabel "Land Use Foundation Theme code list or type"@en .

landUse:attribute a owl:Class,
        skos:Concept ;
    rdfs:label "Land Use Foundation Theme attribute"@en ;
    skos:inScheme ksa-ft:LandUse ;
    skos:prefLabel "Land Use Foundation Theme attribute"@en .

ksa-ft:LandUse a skos:ConceptScheme ;
    rdfs:label "Land Use Foundation Theme"@en ;
    skos:definition "The Land Use Foundation Theme describes human activities in the built and natural environments and includes both existing and future uses of land and natural resources."@en ;
    skos:prefLabel "Land Use Foundation Theme"@en .

