@prefix ksa-ft: <https://w3id.org/ksa/feature-types/> .
@prefix ogc-ft: <http://www.opengis.net/def/metamodel/featuretypes/> .
@prefix owl: <http://www.w3.org/2002/07/owl#> .
@prefix rdfs: <http://www.w3.org/2000/01/rdf-schema#> .
@prefix skos: <http://www.w3.org/2004/02/skos/core#> .
@prefix xsd: <http://www.w3.org/2001/XMLSchema#> .

ksa-ft:DateType a owl:Class,
        skos:Concept ;
    rdfs:label "Date Type"@en ;
    skos:broader <https://w3id.org/ksa/feature-types/LandUse/codeLists> ;
    skos:definition "Reference date and event of lifecycle/process stage of spatial plan document used to describe it."@en ;
    skos:inScheme ksa-ft:LandUse ;
    skos:prefLabel "Date Type"@en .

ksa-ft:LandUseClassificationValue a owl:Class,
        skos:Concept ;
    rdfs:label "Land Use Classification"@en ;
    skos:broader <https://w3id.org/ksa/feature-types/LandUse/codeLists> ;
    skos:definition "List of land use classes to be used in The Kingdom."@en ;
    skos:inScheme ksa-ft:LandUse ;
    skos:prefLabel "Land Use Classification"@en .

ksa-ft:LandUsePercentage a owl:Class,
        skos:Concept ;
    rdfs:label "Land Use Percentage"@en ;
    skos:broader <https://w3id.org/ksa/feature-types/LandUse/codeLists> ;
    skos:definition "Percentage of a land use object that is covered by a presence."@en ;
    skos:inScheme ksa-ft:LandUse ;
    skos:prefLabel "Land Use Percentage"@en .

ksa-ft:OwnershipTypeValue a owl:Class,
        skos:Concept ;
    rdfs:label "Ownership Type"@en ;
    skos:broader <https://w3id.org/ksa/feature-types/LandUse/codeLists> ;
    skos:definition "Type of ownership."@en ;
    skos:inScheme ksa-ft:LandUse ;
    skos:prefLabel "Ownership Type"@en .

ksa-ft:ParcelLandUseValue a owl:Class,
        skos:Concept ;
    rdfs:label "Parcel Land Use Value"@en ;
    skos:broader <https://w3id.org/ksa/feature-types/LandUse/codeLists> ;
    skos:definition "Land Use information within the parcel object."@en ;
    skos:inScheme ksa-ft:LandUse ;
    skos:prefLabel "Parcel Land Use Value"@en .

ksa-ft:ProcessStepGeneralValue a owl:Class,
        skos:Concept ;
    rdfs:label "Process Step General"@en ;
    skos:broader <https://w3id.org/ksa/feature-types/LandUse/codeLists> ;
    skos:definition "General indication of the step of the planning process that the plan is undergoing."@en ;
    skos:inScheme ksa-ft:LandUse ;
    skos:prefLabel "Process Step General"@en .

ksa-ft:RegulationNatureValue a owl:Class,
        skos:Concept ;
    rdfs:label "Regulation Nature"@en ;
    skos:broader <https://w3id.org/ksa/feature-types/LandUse/codeLists> ;
    skos:inScheme ksa-ft:LandUse ;
    skos:prefLabel "Regulation Nature"@en .

ksa-ft:RoadSurfaceCategoryValue a owl:Class,
        skos:Concept ;
    rdfs:label "Road Surface Catagory"@en ;
    skos:broader <https://w3id.org/ksa/feature-types/LandUse/codeLists> ;
    skos:definition "Values to indicate whether a road is paved or not paved."@en ;
    skos:inScheme ksa-ft:LandUse ;
    skos:prefLabel "Road Surface Catagory"@en .

ksa-ft:SpatialPlanTypeValue a owl:Class,
        skos:Concept ;
    rdfs:label "Spatial Plan Type"@en ;
    skos:broader <https://w3id.org/ksa/feature-types/LandUse/codeLists> ;
    skos:definition "Type of spatial plan document."@en ;
    skos:inScheme ksa-ft:LandUse ;
    skos:prefLabel "Spatial Plan Type"@en .

ksa-ft:UrbanBoundaryTypeValue a owl:Class,
        skos:Concept ;
    rdfs:label "Urban Boundary Type"@en ;
    skos:broader <https://w3id.org/ksa/feature-types/LandUse/codeLists> ;
    skos:definition "Type of urban boundary."@en ;
    skos:inScheme ksa-ft:LandUse ;
    skos:prefLabel "Urban Boundary Type"@en .

ksa-ft:VerticalLandUse a owl:Class,
        skos:Concept ;
    rdfs:label "Vertical Land Use"@en ;
    skos:broader <https://w3id.org/ksa/feature-types/LandUse/codeLists> ;
    skos:definition "Land Use classes that are present in a specific vertical level of using of a parcel object."@en ;
    skos:inScheme ksa-ft:LandUse ;
    skos:prefLabel "Vertical Land Use"@en .

ksa-ft:VerticalLevelValue a owl:Class,
        skos:Concept ;
    rdfs:label "Vertical Level"@en ;
    skos:broader <https://w3id.org/ksa/feature-types/LandUse/codeLists> ;
    skos:definition "The relative vertical level of a land use of a parcel object."@en ;
    skos:inScheme ksa-ft:LandUse ;
    skos:prefLabel "Vertical Level"@en .

<https://w3id.org/ksa/feature-types/LandUse/attribute/additionalDescription> a owl:ObjectProperty,
        skos:Concept ;
    rdfs:label "additionalDescription"@en ;
    rdfs:domain ksa-ft:MapDocument ;
    rdfs:subClassOf <https://w3id.org/ksa/feature-types/LandUse/attribute> ;
    skos:broader <https://w3id.org/ksa/feature-types/LandUse/attribute> ;
    skos:definition "Plain text description of additional information not fitting in other attributes."@en ;
    skos:inScheme ksa-ft:LandUse ;
    skos:prefLabel "additionalDescription"@en .

<https://w3id.org/ksa/feature-types/LandUse/attribute/coordinateReferenceSystem> a owl:ObjectProperty,
        skos:Concept ;
    rdfs:label "coordinateReferenceSystem"@en ;
    rdfs:domain ksa-ft:MapDocument ;
    rdfs:subClassOf <https://w3id.org/ksa/feature-types/LandUse/attribute> ;
    skos:broader <https://w3id.org/ksa/feature-types/LandUse/attribute> ;
    skos:definition """Identifier and codespace for coordinate reference system of map document.

NOTE. Refer to EPSG Geodetic Parameter Dataset  (EPSG) as URI identifier of reference system e.g.  http://www.opengis.net/def/crs/EPSG/0/4326"""@en ;
    skos:inScheme ksa-ft:LandUse ;
    skos:prefLabel "coordinateReferenceSystem"@en .

<https://w3id.org/ksa/feature-types/LandUse/attribute/extent> a owl:ObjectProperty,
        skos:Concept ;
    rdfs:label "extent"@en ;
    rdfs:domain ksa-ft:ExistingLandUseCollection ;
    rdfs:subClassOf <https://w3id.org/ksa/feature-types/LandUse/attribute> ;
    skos:broader <https://w3id.org/ksa/feature-types/LandUse/attribute> ;
    skos:definition """Contains the extent of the data set.

NOTE 01. For an area objects boundary of the geometrical union of all the instances of the spatial object type ExistingLandUseUnit.
For an sampled objects the convex hull of all the instances of the spatial object type ExistingLandUseUnit."""@en ;
    skos:inScheme ksa-ft:LandUse ;
    skos:prefLabel "extent"@en .

<https://w3id.org/ksa/feature-types/LandUse/attribute/legend> a owl:ObjectProperty,
        skos:Concept ;
    rdfs:label "legend"@en ;
    rdfs:domain ksa-ft:MapDocument ;
    rdfs:subClassOf <https://w3id.org/ksa/feature-types/LandUse/attribute> ;
    skos:broader <https://w3id.org/ksa/feature-types/LandUse/attribute> ;
    skos:definition "Link to online version of legend of map document."@en ;
    skos:inScheme ksa-ft:LandUse ;
    skos:prefLabel "legend"@en .

<https://w3id.org/ksa/feature-types/LandUse/attribute/link> a owl:ObjectProperty,
        skos:Concept ;
    rdfs:label "link"@en ;
    rdfs:domain ksa-ft:MapDocument ;
    rdfs:subClassOf <https://w3id.org/ksa/feature-types/LandUse/attribute> ;
    skos:broader <https://w3id.org/ksa/feature-types/LandUse/attribute> ;
    skos:definition "Link to online version of map document."@en ;
    skos:inScheme ksa-ft:LandUse ;
    skos:prefLabel "link"@en .

<https://w3id.org/ksa/feature-types/LandUse/attribute/name> a owl:DatatypeProperty,
        skos:Concept ;
    rdfs:label "name"@en ;
    rdfs:domain ksa-ft:ExistingLandUseCollection ;
    rdfs:range xsd:string ;
    rdfs:subClassOf <https://w3id.org/ksa/feature-types/LandUse/attribute> ;
    skos:broader <https://w3id.org/ksa/feature-types/LandUse/attribute> ;
    skos:definition "Name of the Land Use collection"@en ;
    skos:inScheme ksa-ft:LandUse ;
    skos:prefLabel "name"@en .

<https://w3id.org/ksa/feature-types/LandUse/attribute/spatialResolution> a owl:DatatypeProperty,
        skos:Concept ;
    rdfs:label "spatialResolution"@en ;
    rdfs:domain ksa-ft:MapDocument ;
    rdfs:range xsd:integer ;
    rdfs:subClassOf <https://w3id.org/ksa/feature-types/LandUse/attribute> ;
    skos:broader <https://w3id.org/ksa/feature-types/LandUse/attribute> ;
    skos:definition "Level of detail expressed as an integer value expressing the scale denominator of a comparable hardcopy map."@en ;
    skos:inScheme ksa-ft:LandUse ;
    skos:prefLabel "spatialResolution"@en .

<https://w3id.org/ksa/feature-types/LandUse/attribute/title> a owl:DatatypeProperty,
        skos:Concept ;
    rdfs:label "title"@en ;
    rdfs:domain ksa-ft:MapDocument ;
    rdfs:range xsd:string ;
    rdfs:subClassOf <https://w3id.org/ksa/feature-types/LandUse/attribute> ;
    skos:broader <https://w3id.org/ksa/feature-types/LandUse/attribute> ;
    skos:definition "Official title of the map document."@en ;
    skos:inScheme ksa-ft:LandUse ;
    skos:prefLabel "title"@en .

<https://w3id.org/ksa/feature-types/LandUse/attribute/validFrom> a owl:DatatypeProperty,
        skos:Concept ;
    rdfs:label "validFrom"@en ;
    rdfs:domain ksa-ft:ExistingLandUseCollection,
        ksa-ft:MapDocument ;
    rdfs:range xsd:date ;
    rdfs:subClassOf <https://w3id.org/ksa/feature-types/LandUse/attribute> ;
    skos:broader <https://w3id.org/ksa/feature-types/LandUse/attribute> ;
    skos:definition "First date at which the map document is valid in reality."@en,
        "The date when the Land Use data set started to exist in the real world."@en ;
    skos:inScheme ksa-ft:LandUse ;
    skos:prefLabel "validFrom"@en .

<https://w3id.org/ksa/feature-types/LandUse/attribute/validTo> a owl:DatatypeProperty,
        skos:Concept ;
    rdfs:label "validTo"@en ;
    rdfs:domain ksa-ft:ExistingLandUseCollection,
        ksa-ft:MapDocument ;
    rdfs:range xsd:date ;
    rdfs:subClassOf <https://w3id.org/ksa/feature-types/LandUse/attribute> ;
    skos:broader <https://w3id.org/ksa/feature-types/LandUse/attribute> ;
    skos:definition "The dwte from which the Land Use data set no longer exists in the real world."@en,
        "The time from which the map document no longer exists in the real world."@en ;
    skos:inScheme ksa-ft:LandUse ;
    skos:prefLabel "validTo"@en .

ksa-ft:ExistingLandUseCollection a owl:Class,
        skos:Concept ;
    rdfs:label "Existing Land Use Collection"@en ;
    ogc-ft:hasProperty <https://w3id.org/ksa/feature-types/LandUse/attribute/extent>,
        <https://w3id.org/ksa/feature-types/LandUse/attribute/name>,
        <https://w3id.org/ksa/feature-types/LandUse/attribute/validFrom>,
        <https://w3id.org/ksa/feature-types/LandUse/attribute/validTo> ;
    rdfs:subClassOf ksa-ft:AbstractFeatureType ;
    skos:broader ksa-ft:AbstractFeatureType ;
    skos:definition "A collection of units (areas or locations) for which information on existing land use is provided as a polygon."@en ;
    skos:inScheme ksa-ft:LandUse ;
    skos:prefLabel "Existing Land Use Collection"@en .

ksa-ft:MapDocument a owl:Class,
        skos:Concept ;
    rdfs:label "Map Document"@en ;
    ogc-ft:hasProperty <https://w3id.org/ksa/feature-types/LandUse/attribute/additionalDescription>,
        <https://w3id.org/ksa/feature-types/LandUse/attribute/coordinateReferenceSystem>,
        <https://w3id.org/ksa/feature-types/LandUse/attribute/legend>,
        <https://w3id.org/ksa/feature-types/LandUse/attribute/link>,
        <https://w3id.org/ksa/feature-types/LandUse/attribute/spatialResolution>,
        <https://w3id.org/ksa/feature-types/LandUse/attribute/title>,
        <https://w3id.org/ksa/feature-types/LandUse/attribute/validFrom>,
        <https://w3id.org/ksa/feature-types/LandUse/attribute/validTo> ;
    rdfs:subClassOf ksa-ft:AbstractFeatureType ;
    skos:broader ksa-ft:AbstractFeatureType ;
    skos:definition "The scanned plan and structural drawing which may geo-referenced e.g. raster images, vector drawings."@en ;
    skos:inScheme ksa-ft:LandUse ;
    skos:prefLabel "Map Document"@en .

<https://w3id.org/ksa/feature-types/LandUse/codeLists> a owl:Class,
        skos:Concept ;
    rdfs:label "Land Use Foundation Theme code list or type"@en ;
    skos:inScheme ksa-ft:LandUse ;
    skos:prefLabel "Land Use Foundation Theme code list or type"@en .

<https://w3id.org/ksa/feature-types/LandUse/attribute> a owl:Class,
        skos:Concept ;
    rdfs:label "Land Use Foundation Theme attribute"@en ;
    skos:inScheme ksa-ft:LandUse ;
    skos:prefLabel "Land Use Foundation Theme attribute"@en .

ksa-ft:LandUse a skos:ConceptScheme ;
    rdfs:label "Land Use Foundation Theme"@en ;
    skos:definition "The Land Use Foundation Theme describes human activities in the built and natural environments and includes both existing and future uses of land and natural resources."@en ;
    skos:prefLabel "Land Use Foundation Theme"@en .

