@prefix admRegions: <https://w3id.org/ksa/feature-types/AdministrativeRegions/> .
@prefix ksa-ft: <https://w3id.org/ksa/feature-types/> .
@prefix nationalAddress: <https://w3id.org/ksa/feature-types/NationalAddress/> .
@prefix nationalAddress-att: <https://w3id.org/ksa/feature-types/NationalAddress/attribute/> .
@prefix ogc-ft: <http://www.opengis.net/def/metamodel/featuretypes/> .
@prefix owl: <http://www.w3.org/2002/07/owl#> .
@prefix rdfs: <http://www.w3.org/2000/01/rdf-schema#> .
@prefix skos: <http://www.w3.org/2004/02/skos/core#> .
@prefix xsd: <http://www.w3.org/2001/XMLSchema#> .

nationalAddress:AddressLifeCycleStageValue a owl:Class,
        skos:Concept ;
    rdfs:label "AddressLifeCycleStageValue"@en ;
    skos:broader nationalAddress:codeLists ;
    skos:definition "The list defining the stage of the address life."@en ;
    skos:inScheme ksa-ft:NationalAddress ;
    skos:prefLabel "AddressLifeCycleStageValue"@en .

nationalAddress:AddressRepresentation a owl:Class,
        skos:Concept ;
    rdfs:label "Address Representation"@en ;
    skos:broader nationalAddress:codeLists ;
    skos:definition "Representation of an address feature for use in external application schemas that need to include the basic, address information in a readable way.   Attributes are filled from the values from Address and AddressComponent classes."@en ;
    skos:inScheme ksa-ft:NationalAddress ;
    skos:prefLabel "Address Representation"@en .

nationalAddress:POICategoryListValue a owl:Class,
        skos:Concept ;
    rdfs:label "POICategoryListValue"@en ;
    skos:broader nationalAddress:codeLists ;
    skos:definition """List of category names of POI (Point of Interest).

NOTE The list is divided into sub categories and some of categories are divided into sub sub categories."""@en ;
    skos:inScheme ksa-ft:NationalAddress ;
    skos:prefLabel "POICategoryListValue"@en .

nationalAddress-att:coverage a owl:ObjectProperty,
        skos:Concept ;
    rdfs:label "coverage" ;
    rdfs:domain nationalAddress:ZipCodeUnit ;
    rdfs:range admRegions:RegionalAdministrativeUnit ;
    rdfs:subClassOf nationalAddress:attribute ;
    skos:broader nationalAddress:attribute ;
    skos:prefLabel "coverage" .

nationalAddress-att:neighborhood a owl:ObjectProperty,
        skos:Concept ;
    rdfs:label "neighborhood" ;
    rdfs:domain nationalAddress:NonAddressObject ;
    rdfs:range admRegions:PointOfInterest ;
    rdfs:subClassOf nationalAddress:attribute ;
    skos:broader nationalAddress:attribute ;
    skos:prefLabel "neighborhood" .

admRegions:MunicipalAdministrativeUnit a owl:Class,
        skos:Concept ;
    rdfs:label "Municipal Administrative Unit"@en ;
    skos:definition "Spatial hierarchy of municipal administration units, governed by the  Ministry of Municipal and Regional Affairs, that divide areas where legislated local governance rights are exercised."@en ;
    skos:prefLabel "Municipal Administrative Unit"@en .

admRegions:PointOfInterest a owl:Class,
        skos:Concept ;
    rdfs:label "Point Of Interest"@en ;
    skos:definition """Specific point location of a place, feature, building or landmark that is of interest, or useful to, people. This includes different categories of POIs including accommodation, eating and drinking, commercial services, religious sites, culture and heritage, attractions, sport and entertainment, education and health, public infrastructure, manufacturing and production, retail and transport.

Specific point location of a place, feature, building or landmark that is of interest, or useful to, people. This includes different categories of POIs including accommodation, eating, commercial services, religious sites, cultural and heritage, attractions, sport and entertainment, education and health, public infrastructure, manufacturing and production, retail and transport."""@en ;
    skos:prefLabel "Point Of Interest"@en .

admRegions:RegionalAdministrativeUnit a owl:Class,
        skos:Concept ;
    rdfs:label "Regional Administrative Unit"@en ;
    skos:definition "Spatial hierarchy of regional administration units, governed by the Ministry of Interior, that divides areas where legislated regional governance rights are exercised."@en ;
    skos:prefLabel "Regional Administrative Unit"@en .

nationalAddress:CityName a owl:Class,
        skos:Concept ;
    rdfs:label "City Name"@en ;
    ogc-ft:hasProperty nationalAddress-att:name ;
    rdfs:subClassOf nationalAddress:AddressComponent ;
    skos:broader nationalAddress:AddressComponent ;
    skos:definition "An address component which represents the name of city within which are contained all finer address elements including districts / neighborhoods, street names and building numbers.  [Unified National Addressing System]"@en ;
    skos:inScheme ksa-ft:NationalAddress ;
    skos:prefLabel "City Name"@en .

nationalAddress:DistrictName a owl:Class,
        skos:Concept ;
    rdfs:label "District Name"@en ;
    ogc-ft:hasProperty nationalAddress-att:name ;
    rdfs:subClassOf nationalAddress:AddressComponent ;
    skos:broader nationalAddress:AddressComponent ;
    skos:definition "An address component which represents the name of municipal district/neighborhood within which buildings and addresses sit.  [Unified National Addressing System]"@en ;
    skos:inScheme ksa-ft:NationalAddress ;
    skos:prefLabel "District Name"@en .

nationalAddress:ObjectCategoryValue a owl:Class,
        skos:Concept ;
    rdfs:label "ObjectCategoryValue"@en ;
    skos:broader nationalAddress:codeLists ;
    skos:definition "The category that describes the Non-Addressable Object"@en ;
    skos:inScheme ksa-ft:NationalAddress ;
    skos:prefLabel "ObjectCategoryValue"@en .

nationalAddress:ZipCodeHierarchyLevelValue a owl:Class,
        skos:Concept ;
    rdfs:label "zip code hierarchy level"@en ;
    skos:broader nationalAddress:codeLists ;
    skos:inScheme ksa-ft:NationalAddress ;
    skos:prefLabel "zip code hierarchy level"@en .

nationalAddress-att:alternativeId a owl:ObjectProperty,
        skos:Concept ;
    rdfs:label "alternativeId"@en ;
    rdfs:domain nationalAddress:AddressComponent ;
    rdfs:range <https://w3id.org/ksa/feature-types/BaseTypes/ThematicIdentifier> ;
    rdfs:subClassOf nationalAddress:attribute ;
    skos:broader nationalAddress:attribute ;
    skos:definition "External, thematic identifier of the address spatial object, which enables interoperability with existing legacy systems or applications."@en ;
    skos:inScheme ksa-ft:NationalAddress ;
    skos:prefLabel "alternativeId"@en .

nationalAddress-att:category a owl:ObjectProperty,
        skos:Concept ;
    rdfs:label "category"@en ;
    rdfs:domain nationalAddress:NonAddressObject ;
    rdfs:range nationalAddress:ObjectCategoryValue ;
    rdfs:subClassOf nationalAddress:attribute ;
    skos:broader nationalAddress:attribute ;
    skos:definition """Describes the type of Non Addressable Object. Defined by codelist ObjectCategoryValue. This has a type and subtype. 

NOTE this codelist is still being developed with the Data Custodian and as of 01/12/2019, the a proposal has been submitted for the high level categories."""@en ;
    skos:inScheme ksa-ft:NationalAddress ;
    skos:prefLabel "category"@en .

nationalAddress-att:codeNumber a owl:DatatypeProperty,
        skos:Concept ;
    rdfs:label "codeNumber"@en ;
    rdfs:domain nationalAddress:ZipCodeUnit ;
    rdfs:range xsd:integer ;
    rdfs:subClassOf nationalAddress:attribute ;
    skos:broader nationalAddress:attribute ;
    skos:definition "The number of the level in the postcode Hierarchy. For example, Riyadh is the number 1."@en ;
    skos:inScheme ksa-ft:NationalAddress ;
    skos:prefLabel "codeNumber"@en .

nationalAddress-att:extent a owl:ObjectProperty,
        skos:Concept ;
    rdfs:label "extent"@en ;
    rdfs:domain nationalAddress:ZipCodeUnit ;
    rdfs:subClassOf nationalAddress:attribute ;
    skos:broader nationalAddress:attribute ;
    skos:inScheme ksa-ft:NationalAddress ;
    skos:prefLabel "extent"@en .

nationalAddress-att:levelName a owl:DatatypeProperty,
        skos:Concept ;
    rdfs:label "levelName"@en ;
    rdfs:domain nationalAddress:ZipCodeUnit ;
    rdfs:range xsd:string ;
    rdfs:subClassOf nationalAddress:attribute ;
    skos:broader nationalAddress:attribute ;
    skos:definition "The name of the level. For example: 1 = \"Region\""@en ;
    skos:inScheme ksa-ft:NationalAddress ;
    skos:prefLabel "levelName"@en .

nationalAddress-att:location a owl:ObjectProperty,
        skos:Concept ;
    rdfs:label "location"@en ;
    rdfs:domain nationalAddress:NonAddressObject ;
    rdfs:subClassOf nationalAddress:attribute ;
    skos:broader nationalAddress:attribute ;
    skos:definition "The location (coordinates in the coordinate reference system) of the Non Addressable Object."@en ;
    skos:inScheme ksa-ft:NationalAddress ;
    skos:prefLabel "location"@en .

nationalAddress-att:zipCodeLevel a owl:ObjectProperty,
        skos:Concept ;
    rdfs:label "zipCodeLevel"@en ;
    rdfs:domain nationalAddress:ZipCodeUnit ;
    rdfs:range nationalAddress:ZipCodeHierarchyLevelValue ;
    rdfs:subClassOf nationalAddress:attribute ;
    skos:broader nationalAddress:attribute ;
    skos:definition "The level in the postcode hierarchy. 1st Order, second order etc."@en ;
    skos:inScheme ksa-ft:NationalAddress ;
    skos:prefLabel "zipCodeLevel"@en .

nationalAddress-att:name a owl:DatatypeProperty,
        owl:ObjectProperty,
        skos:Concept ;
    rdfs:label "name",
        "name"@en ;
    rdfs:domain nationalAddress:CityName,
        nationalAddress:DistrictName ;
    rdfs:range xsd:string,
        admRegions:MunicipalAdministrativeUnit ;
    rdfs:subClassOf nationalAddress:attribute ;
    skos:broader nationalAddress:attribute ;
    skos:definition "Name of the city."@en,
        "Name of the district."@en ;
    skos:inScheme ksa-ft:NationalAddress ;
    skos:prefLabel "name",
        "name"@en .

nationalAddress-att:validFrom a owl:DatatypeProperty,
        skos:Concept ;
    rdfs:label "validFrom"@en ;
    rdfs:domain nationalAddress:AddressComponent,
        nationalAddress:ZipCodeUnit ;
    rdfs:range xsd:date ;
    rdfs:subClassOf nationalAddress:attribute ;
    skos:broader nationalAddress:attribute ;
    skos:definition "Date of the address component was or will be valid in the real world."@en,
        "Date of which this version of the Postal Code Unit was or will be valid in the real world."@en ;
    skos:inScheme ksa-ft:NationalAddress ;
    skos:prefLabel "validFrom"@en .

nationalAddress-att:validTo a owl:DatatypeProperty,
        skos:Concept ;
    rdfs:label "validTo"@en ;
    rdfs:domain nationalAddress:AddressComponent,
        nationalAddress:ZipCodeUnit ;
    rdfs:range xsd:date ;
    rdfs:subClassOf nationalAddress:attribute ;
    skos:broader nationalAddress:attribute ;
    skos:definition "Date at which this version of the Postal Code Unit ceased or will cease to exist in the real world."@en,
        "Date at which this version of the address component ceased or will cease to exist in the real world."@en ;
    skos:inScheme ksa-ft:NationalAddress ;
    skos:prefLabel "validTo"@en .

nationalAddress:NonAddressObject a owl:Class,
        skos:Concept ;
    rdfs:label "Non-Addressable Object"@en ;
    ogc-ft:hasProperty nationalAddress-att:category,
        nationalAddress-att:location ;
    rdfs:subClassOf <https://w3id.org/ksa/feature-types/BaseTypes/AbstractFeatureType> ;
    skos:broader <https://w3id.org/ksa/feature-types/BaseTypes/AbstractFeatureType> ;
    skos:definition "Physical, visible and stationary objects that are representable as point locations, that you cannot send mail to, and are not classified as a Point of Interest. Non Addressable Objects (NAOs) may have a link to the nearest address."@en ;
    skos:inScheme ksa-ft:NationalAddress ;
    skos:prefLabel "Non-Addressable Object"@en .

nationalAddress:codeLists a owl:Class,
        skos:Concept ;
    rdfs:label "National Address Foundation Theme code list or type"@en ;
    skos:inScheme ksa-ft:NationalAddress ;
    skos:prefLabel "National Address Foundation Theme code list or type"@en .

nationalAddress:AddressComponent a owl:Class,
        skos:Concept ;
    rdfs:label "Address Component"@en ;
    ogc-ft:hasProperty nationalAddress-att:alternativeId,
        nationalAddress-att:validFrom,
        nationalAddress-att:validTo ;
    rdfs:subClassOf <https://w3id.org/ksa/feature-types/BaseTypes/AbstractFeatureType> ;
    skos:broader <https://w3id.org/ksa/feature-types/BaseTypes/AbstractFeatureType> ;
    skos:definition "Identifier, code or geographic name of a specific geographic area, location, or other spatial object which defines the scope of an address."@en ;
    skos:inScheme ksa-ft:NationalAddress ;
    skos:prefLabel "Address Component"@en .

nationalAddress:ZipCodeUnit a owl:Class,
        skos:Concept ;
    rdfs:label "Zip Code Unit"@en ;
    ogc-ft:hasProperty nationalAddress-att:codeNumber,
        nationalAddress-att:extent,
        nationalAddress-att:levelName,
        nationalAddress-att:validFrom,
        nationalAddress-att:validTo,
        nationalAddress-att:zipCodeLevel ;
    rdfs:subClassOf <https://w3id.org/ksa/feature-types/BaseTypes/AbstractFeatureType> ;
    skos:broader <https://w3id.org/ksa/feature-types/BaseTypes/AbstractFeatureType> ;
    skos:definition "A code created and maintained for postal purposes to identify a subdivision of addresses and postal delivery points."@en ;
    skos:inScheme ksa-ft:NationalAddress ;
    skos:prefLabel "Zip Code Unit"@en .

ksa-ft:NationalAddress a skos:ConceptScheme ;
    rdfs:label "National Address Foundation Theme"@en ;
    skos:definition "The National Address Foundation Theme is a unified location identification Foundation Theme, in the form of a geocoded structured label, for properties, non-addressable objects and points of interest. Labels contain building numbers, street names, district names, city names, zip codes, additional and unit numbers."@en ;
    skos:prefLabel "National Address Foundation Theme"@en .

nationalAddress:attribute a owl:Class,
        skos:Concept ;
    rdfs:label "National Address Foundation Theme attribute"@en ;
    skos:inScheme ksa-ft:NationalAddress ;
    skos:prefLabel "National Address Foundation Theme attribute"@en .

