@prefix ksa-ft: <https://w3id.org/ksa/feature-types/> .
@prefix ogc-ft: <http://www.opengis.net/def/metamodel/featuretypes/> .
@prefix owl: <http://www.w3.org/2002/07/owl#> .
@prefix rdfs: <http://www.w3.org/2000/01/rdf-schema#> .
@prefix skos: <http://www.w3.org/2004/02/skos/core#> .

ksa-ft:DitchTypeValue a owl:Class,
        skos:Concept ;
    rdfs:label "Ditch Type Value"@en ;
    skos:broader <https://w3id.org/ksa/feature-types/Water/codeLists> ;
    skos:definition "A coded domain value denoting a ditch type (e.g. roadside or irrigation ditch)."@en ;
    skos:inScheme ksa-ft:Water .

ksa-ft:HydroNodeCategoryValue a owl:Class,
        skos:Concept ;
    rdfs:label "Hydro Node Category Value"@en ;
    skos:broader <https://w3id.org/ksa/feature-types/Water/codeLists> ;
    skos:definition "Defines categories for different types of hydrographic network nodes."@en ;
    skos:inScheme ksa-ft:Water .

ksa-ft:HydroOrderCode a owl:Class,
        skos:Concept ;
    rdfs:label "Hydro Order Code"@en ;
    skos:broader <https://w3id.org/ksa/feature-types/Water/codeLists> ;
    skos:definition "A hydrologically meaningful 'order code' for ordering hierarchies of watercourses and drainage basins."@en ;
    skos:inScheme ksa-ft:Water .

ksa-ft:HydrologicalPersistenceValue a owl:Class,
        skos:Concept ;
    rdfs:label "Hydrological Persistence Value"@en ;
    skos:broader <https://w3id.org/ksa/feature-types/Water/codeLists> ;
    skos:definition "Categories of hydrological persistence of a body of water."@en ;
    skos:inScheme ksa-ft:Water .

ksa-ft:SeaAreaTypeClassificationValue a owl:Class,
        skos:Concept ;
    rdfs:label "Sea Area Type Classification Value"@en ;
    skos:broader <https://w3id.org/ksa/feature-types/Water/codeLists> ;
    skos:definition "Classification type of the SeaArea (e.g. estuary, openOcean)."@en ;
    skos:inScheme ksa-ft:Water .

ksa-ft:SeaSurfaceClassificationValue a owl:Class,
        skos:Concept ;
    rdfs:label "Sea Surface Classification Value"@en ;
    skos:broader <https://w3id.org/ksa/feature-types/Water/codeLists> ;
    skos:definition "Types of sea surface layers found on sea surfaces."@en ;
    skos:inScheme ksa-ft:Water .

ksa-ft:SeabedCoverValue a owl:Class,
        skos:Concept ;
    rdfs:label "Seabed Cover Value"@en ;
    skos:broader <https://w3id.org/ksa/feature-types/Water/codeLists> ;
    skos:definition "Types of cover found on sea beds."@en ;
    skos:inScheme ksa-ft:Water .

ksa-ft:ShoreStabilityValue a owl:Class,
        skos:Concept ;
    rdfs:label "Shore Stability Value"@en ;
    skos:broader <https://w3id.org/ksa/feature-types/Water/codeLists> ;
    skos:definition "Types of the stability of shore segments."@en ;
    skos:inScheme ksa-ft:Water .

ksa-ft:ShoreTypeClassificationValue a owl:Class,
        skos:Concept ;
    rdfs:label "Shore Type Classification Value"@en ;
    skos:broader <https://w3id.org/ksa/feature-types/Water/codeLists> ;
    skos:definition "The allowed values for this code list comprise any values defined by data providers."@en ;
    skos:inScheme ksa-ft:Water .

ksa-ft:ShoreTypeValue a owl:Class,
        skos:Concept ;
    rdfs:label "Shore Type Value"@en ;
    skos:broader <https://w3id.org/ksa/feature-types/Water/codeLists> ;
    skos:definition "Categories of shore area composition."@en ;
    skos:inScheme ksa-ft:Water .

<https://w3id.org/ksa/feature-types/Water/attribute/relatedRepresentation> a owl:ObjectProperty,
        skos:Concept ;
    rdfs:label "relatedRepresentation" ;
    rdfs:domain ksa-ft:AbstractHydroFeature ;
    rdfs:range ksa-ft:AbstractHydroFeature ;
    rdfs:subClassOf <https://w3id.org/ksa/feature-types/Water/attribute> ;
    skos:broader <https://w3id.org/ksa/feature-types/Water/attribute> .

ksa-ft:ZoneTypeValue a owl:Class,
        skos:Concept ;
    rdfs:label "Zone Type Value"@en ;
    skos:broader <https://w3id.org/ksa/feature-types/Water/codeLists> ;
    skos:definition "Types of marine circulation zones."@en ;
    skos:inScheme ksa-ft:Water .

ksa-ft:OriginValue a owl:Class,
        skos:Concept ;
    rdfs:label "Origin Value"@en ;
    skos:broader <https://w3id.org/ksa/feature-types/Water/codeLists> ;
    skos:definition "An enumeration type specifying a set of hydrographic 'origin' categories (natural, man-made) for various hydrographic objects."@en ;
    skos:inScheme ksa-ft:Water .

<https://w3id.org/ksa/feature-types/Water/attribute/centerline> a owl:ObjectProperty,
        skos:Concept ;
    rdfs:label "centerline"@en ;
    rdfs:domain ksa-ft:LandWaterBoundary ;
    rdfs:subClassOf <https://w3id.org/ksa/feature-types/Water/attribute> ;
    skos:broader <https://w3id.org/ksa/feature-types/Water/attribute> ;
    skos:definition "The geometry of the land-water boundary, as a curve."@en ;
    skos:inScheme ksa-ft:Water .

<https://w3id.org/ksa/feature-types/Water/attribute/extent> a owl:ObjectProperty,
        skos:Concept ;
    rdfs:label "extent"@en ;
    rdfs:domain ksa-ft:AbstractMarineLayer ;
    rdfs:subClassOf <https://w3id.org/ksa/feature-types/Water/attribute> ;
    skos:broader <https://w3id.org/ksa/feature-types/Water/attribute> ;
    skos:definition "Geometry of the marine layer."@en ;
    skos:inScheme ksa-ft:Water .

<https://w3id.org/ksa/feature-types/Water/attribute/geographicalName> a owl:ObjectProperty,
        skos:Concept ;
    rdfs:label "geographicalName"@en ;
    rdfs:domain ksa-ft:WatercourseSeparatedCrossing ;
    rdfs:range ksa-ft:GeographicalName ;
    rdfs:subClassOf <https://w3id.org/ksa/feature-types/Water/attribute> ;
    skos:broader <https://w3id.org/ksa/feature-types/Water/attribute> ;
    skos:definition "A geographical name that is used to identify a water course separated crossing."@en ;
    skos:inScheme ksa-ft:Water .

<https://w3id.org/ksa/feature-types/Water/attribute/name> a owl:ObjectProperty,
        skos:Concept ;
    rdfs:label "name"@en ;
    rdfs:domain ksa-ft:AbstractHydroFeature ;
    rdfs:range ksa-ft:GeographicalName ;
    rdfs:subClassOf <https://w3id.org/ksa/feature-types/Water/attribute> ;
    skos:broader <https://w3id.org/ksa/feature-types/Water/attribute> ;
    skos:definition "The name or names by which a hydrographic feature is knowng in the real world. This can act as an implicit identifier for different spatial representations of the same real-world feature."@en ;
    skos:inScheme ksa-ft:Water .

<https://w3id.org/ksa/feature-types/Water/attribute/origin> a owl:ObjectProperty,
        skos:Concept ;
    rdfs:label "origin"@en ;
    rdfs:domain ksa-ft:LandWaterBoundary ;
    rdfs:range ksa-ft:OriginValue ;
    rdfs:subClassOf <https://w3id.org/ksa/feature-types/Water/attribute> ;
    skos:broader <https://w3id.org/ksa/feature-types/Water/attribute> ;
    skos:definition "Origin of the land-water boundary."@en ;
    skos:inScheme ksa-ft:Water .

<https://w3id.org/ksa/feature-types/Water/attribute/validTime> a owl:ObjectProperty,
        skos:Concept ;
    rdfs:label "validTime"@en ;
    rdfs:domain ksa-ft:AbstractMarineLayer ;
    rdfs:subClassOf <https://w3id.org/ksa/feature-types/Water/attribute> ;
    skos:broader <https://w3id.org/ksa/feature-types/Water/attribute> ;
    skos:definition "Time period for which the marine layer is valid."@en ;
    skos:inScheme ksa-ft:Water .

<https://w3id.org/ksa/feature-types/Water/attribute/waterLevelCategory> a owl:ObjectProperty,
        skos:Concept ;
    rdfs:label "waterLevelCategory"@en ;
    rdfs:domain ksa-ft:LandWaterBoundary ;
    rdfs:range ksa-ft:WaterLevelValue ;
    rdfs:subClassOf <https://w3id.org/ksa/feature-types/Water/attribute> ;
    skos:broader <https://w3id.org/ksa/feature-types/Water/attribute> ;
    skos:definition "Water-level defining the land-water boundary."@en ;
    skos:inScheme ksa-ft:Water .

ksa-ft:WaterLevelValue a owl:Class,
        skos:Concept ;
    rdfs:label "Water Level Value"@en ;
    skos:broader <https://w3id.org/ksa/feature-types/Water/codeLists> ;
    skos:definition "The tidal datum / waterlevel to which depths and heights are referenced."@en ;
    skos:inScheme ksa-ft:Water .

ksa-ft:AbstractMarineLayer a owl:Class,
        skos:Concept ;
    rdfs:label "Abstract Marine Layer"@en ;
    ogc-ft:hasProperty <https://w3id.org/ksa/feature-types/Water/attribute/extent>,
        <https://w3id.org/ksa/feature-types/Water/attribute/validTime> ;
    rdfs:subClassOf ksa-ft:AbstractHydroFeature ;
    skos:broader ksa-ft:AbstractHydroFeature ;
    skos:definition "A layer that may cover any part of a sea surface or sea bottom, represented as either a surface or point. The point representation reflects the reality that many Marine Layers are identified by point observations."@en ;
    skos:inScheme ksa-ft:Water .

<https://w3id.org/ksa/feature-types/Water/attribute/hydroID> a owl:ObjectProperty,
        skos:Concept ;
    rdfs:label "hydroID"@en ;
    rdfs:domain ksa-ft:AbstractHydroFeature,
        ksa-ft:WatercourseSeparatedCrossing ;
    rdfs:subClassOf <https://w3id.org/ksa/feature-types/Water/attribute> ;
    skos:broader <https://w3id.org/ksa/feature-types/Water/attribute> ;
    skos:definition "A hydrographic thematic identifier, for example, a Data Owner internal identifier."@en ;
    skos:inScheme ksa-ft:Water .

ksa-ft:WatercourseSeparatedCrossing a owl:Class,
        skos:Concept ;
    rdfs:label "Watercourse Separated Crossing"@en ;
    ogc-ft:hasProperty <https://w3id.org/ksa/feature-types/Water/attribute/geographicalName>,
        <https://w3id.org/ksa/feature-types/Water/attribute/hydroID> ;
    rdfs:subClassOf ksa-ft:GradeSeparatedCrossing ;
    skos:broader ksa-ft:GradeSeparatedCrossing ;
    skos:definition "An element in the hydrographic network used to indicate non-interacting crossing of watercourse links separated by level."@en ;
    skos:inScheme ksa-ft:Water .

ksa-ft:LandWaterBoundary a owl:Class,
        skos:Concept ;
    rdfs:label "Land Water Boundary"@en ;
    ogc-ft:hasProperty <https://w3id.org/ksa/feature-types/Water/attribute/centerline>,
        <https://w3id.org/ksa/feature-types/Water/attribute/origin>,
        <https://w3id.org/ksa/feature-types/Water/attribute/waterLevelCategory> ;
    rdfs:subClassOf ksa-ft:AbstractFeatureType ;
    skos:broader ksa-ft:AbstractFeatureType ;
    skos:definition "The line where a land mass is in contact with a body of water."@en ;
    skos:inScheme ksa-ft:Water .

ksa-ft:AbstractHydroFeature a owl:Class,
        skos:Concept ;
    rdfs:label "Abstract Hydro Feature"@en ;
    ogc-ft:hasProperty <https://w3id.org/ksa/feature-types/Water/attribute/hydroID>,
        <https://w3id.org/ksa/feature-types/Water/attribute/name> ;
    rdfs:subClassOf ksa-ft:AbstractFeatureType ;
    skos:broader ksa-ft:AbstractFeatureType ;
    skos:definition "This base abstract hydrographic class enables associations between different hydrographic feature instances representing the same real world entity. Three mechanisms are provided for this: a shared name attribute that allows an implicit association on the basis of a common name; a shared hydroID attribute where multiple representations are explicitly identified as the same instance; an explicit association between feature instances representing the same real-world entity."@en ;
    skos:inScheme ksa-ft:Water .

<https://w3id.org/ksa/feature-types/Water/codeLists> a owl:Class,
        skos:Concept ;
    rdfs:label "Water Foundation Theme code list or type"@en ;
    skos:inScheme ksa-ft:Water .

<https://w3id.org/ksa/feature-types/Water/attribute> a owl:Class,
        skos:Concept ;
    rdfs:label "Water Foundation Theme attribute"@en ;
    skos:inScheme ksa-ft:Water .

ksa-ft:Water a skos:ConceptScheme ;
    rdfs:label "Water Foundation Theme"@en ;
    skos:definition "The Water Foundation Theme depicts and specifies all surface water types and water resources including perpetual and transient water courses, artificial surface water bodies, and sea water. While it includes all water features that are intrinsic to (part of) a surface water hydrological network, it excludes ultimate uses of water such as irrigation and waterborne transport."@en .

